AP/AP/HistBlind/D.lean
@@ -2,9 +2,6 @@ import AP.AP.HistBlind.A
 
 namespace AP
 
-instance : (default : DStrat).histBlind := by
-  simp [DStrat.histBlind]
-
 noncomputable
 def State.dwn (s : State) : ℕ :=
   Nat.findRaw # λ n => ∃ (d : DStrat), d.WF ∧ ∀ (a : AStrat), a.WF →
@@ -117,7 +114,7 @@ theorem State.dwn_setHist {s hist} [hs : sys.WF s] [hs' : sys.WF # s.setHist his
       exact System.reachable_of_simulate_full H₂
     simp [setHistAt, H₆, H₆', H₈, H₈'] at H₄ H₄'
     have G₁ : sys.tr s₁' (d.f s₁) = some s₂'
-    · simp [-DState.tr_eq_some_iff, ←hd', H₄, setHistAt, H₈', hs₁.wf_s] at H₅
+    · simp [-DState.tr_eq_some_iff, ←hd', H₄, setHistAt, H₈', hs₁.wf] at H₅
       replace H₅ : sys.tr s₁' (((guard (f := Option)
         (sys.validTr (s₁.setHistAt' s.hist s'.hist) (d.f s₁))).bind #
         λ x => some (d.f s₁)).getD s₁'.chooseDMove) = some s₂'
@@ -140,14 +137,253 @@ theorem State.dwn_setHist {s hist} [hs : sys.WF s] [hs' : sys.WF # s.setHist his
     simp
     exact List.IsSuffix.length_le H₈'
 
+theorem State.a_hws_of_dwn_eq_zero {s} [hs : sys.WF s]
+(h : s.dwn = 0) : s.a_hws := by
+  by_contra h₁
+  simp at h₁
+  rw [d_hws_iff_d_hws_bounded] at h₁
+  replace h₁ := Nat.findRaw_spec' h₁
+  rw [←dwn] at h₁
+  simp [h] at h₁
+  exact h₁.2 default inferInstance
+
+theorem State.dwn_eq_zero_iff_a_hws {s} [hs : sys.WF s] : s.dwn = 0 ↔ s.a_hws :=
+  ⟨a_hws_of_dwn_eq_zero, dwn_eq_zero_of_a_hws⟩
+
+theorem State.d_hws_iff_dwn_ne_zero {s} [hs : sys.WF s] : s.d_hws ↔ s.dwn ≠ 0 := by
+  simp [dwn_eq_zero_iff_a_hws]
+
+theorem State.dwn_pos_of_d_hws {s} [hs : sys.WF s] (h : s.d_hws) : 0 < s.dwn := by
+  simpa [zero_lt_iff, dwn_eq_zero_iff_a_hws]
+
+theorem AState.dwn_lt_of_tr {sa sd p} [hsa : AState sa]
+(h₁ : sa.d_hws) (h₂ : sys.tr sa p = some sd) : sd.dwn < sa.dwn := by
+  have hsd := sys.wf_of_tr h₂
+  have h₃ := d_hws_of_tr h₂ h₁
+  have hp₁ := State.dwn_pos_of_d_hws h₁
+  rw [State.d_hws_iff_d_hws_bounded] at h₁ h₃
+  replace h₁ := Nat.findRaw_spec' h₁
+  replace h₃ := Nat.findRaw_spec' h₃
+  rw [←State.dwn] at h₁ h₃
+  generalize hn : sa.dwn = n at h₁ h₃ hp₁ ⊢
+  generalize hn' : sd.dwn = n' at h₁ h₃ hp₁ ⊢
+  obtain ⟨⟨d, Hd, h₁⟩, h₄⟩ := h₁
+  replace h₃ := h₃.2
+  by_contra! h₅
+  specialize h₃ (n - 1) _
+  rotate_left; contrapose! h₃; cases n; simp at hp₁; simpa
+  clear h₃
+  use d, Hd
+  intro a Ha
+  specialize h₁ (a.set sa p) # a.wf_set_of_tr h₂
+  contrapose! h₁
+  cases n; simp at hp₁; nm n
+  dsimp at h₁
+  simp [h₂]
+  convert h₁ using 2
+  apply simulate_set_a_eq_of_length_hist_lt ⟨_, h₂⟩
+  exact State.length_hist_lt_of_tr h₂
+
+theorem DState.exi_dwn_lt_tr {sd} [hsd : DState sd]
+(h₁ : sd.d_hws) : ∃ p sa, sys.tr sd p = some sa ∧ sa.dwn < sd.dwn := by
+  have hp₁ := State.dwn_pos_of_d_hws h₁
+  rw [State.d_hws_iff_d_hws_bounded] at h₁
+  replace h₁ := Nat.findRaw_spec' h₁
+  rw [←State.dwn] at h₁
+  rcases h₁ with ⟨⟨d, Hd, h₁⟩, h₂⟩
+  obtain ⟨sa, h₃⟩ := Hd.validTr sd
+  use d.f sd, sa, h₃
+  generalize hn : sd.dwn = n at h₁ h₂ hp₁ ⊢
+  have hsa := AState.of_tr h₃
+  have h₄ : sa.d_hws
+  · use d, Hd
+    intro a Ha
+    specialize h₁ a Ha
+    use n - 1
+    cases n; simp at hp₁; nm n
+    simp [h₃] at h₁
+    exact h₁
+  rw [State.d_hws_iff_d_hws_bounded] at h₄
+  replace h₄ := Nat.findRaw_spec' h₄
+  rw [←State.dwn] at h₄
+  generalize hn' : sa.dwn = n' at h₁ h₂ hp₁ h₄ ⊢
+  rcases h₄ with ⟨h₄, h₅⟩
+  by_contra! h₆
+  specialize h₅ (n - 1) _
+  rotate_left; cases n; simp at hp₁; omega
+  clear h₅
+  obtain ⟨d', Hd', h₄⟩ := h₄
+  use d, Hd
+  intro a Ha
+  specialize h₁ a Ha
+  contrapose! h₁
+  cases n; simp at hp₁; nm n
+  simpa [h₃]
+
+open Classical in noncomputable
+def dHistBlind : DStrat := .mk' # λ s => do
+  let sd ← choose? # λ (sd : State) => sd.WF ∧ sd.setHist s.hist = s
+  choose? # λ p => ∃ sa, sys.tr sd p = some sa ∧ sa.d_hws ∧ sa.dwn < sd.dwn
+
+instance : dHistBlind.WF := by unfold dHistBlind; infer_instance
+
+theorem histBlind_dHistBlind : dHistBlind.HistBlind := by
+  use inferInstance
+  intro s hist hs hs' h₁
+  have h₂ : ∃ (sd : State), sd.WF ∧ sd.setHist hist = s.setHist hist; use s, hs.wf
+  generalize h₃ : Classical.epsilon (λ (sd : State) =>
+    sd.WF ∧ sd.setHist hist = s.setHist hist) = sd
+  have h₄ := Classical.epsilon_spec h₂
+  rw [h₃] at h₄
+  rcases h₄ with ⟨hsd, h₄⟩
+  replace hsd : DState sd
+  · use hsd
+    apply congrArg (·.setHist sd.hist) at h₄
+    simp at h₄
+    rw [h₄]
+    simp
+  have h₅ : ∃ (sd : State), sd.WF ∧sd.setHist s.hist = s; use s, hs.wf; simp
+  generalize h₆ : Classical.epsilon (λ (sd : State) =>
+    sd.WF ∧ sd.setHist s.hist = s) = sd'
+  have h₇ := Classical.epsilon_spec h₅
+  rw [h₆] at h₇
+  rcases h₇ with ⟨hsd', h₇⟩
+  replace hsd' : DState sd'
+  · use hsd'
+    apply congrArg (·.setHist sd'.hist) at h₇
+    simp at h₇
+    rw [h₇]
+    simp
+  simp [-DState.tr_eq_some_iff, dHistBlind, choose?_eq_ite, h₃, h₅, h₆]
+  have h₇' := setHist_eq_comm.mp h₇
+  have H₃ : sd.setHist s.hist = s
+  · apply congrArg (·.setHist s.hist) at h₄
+    simp at h₄
+    exact h₄
+  have H₆ : sd.setHist sd'.hist = sd'
+  · trans s.setHist sd'.hist
+    rotate_left; exact h₇'
+    apply congrArg (·.setHist sd'.hist) at h₄
+    simp at h₄
+    exact h₄
+  have H₃' := setHist_eq_comm.mp H₃
+  have h₈ : ∀ p, (∃ sa, sys.tr sd p = some sa ∧ sa.d_hws ∧ sa.dwn < sd.dwn) ↔
+    ∃ sa, sys.tr sd' p = some sa ∧ sa.d_hws ∧ sa.dwn < sd'.dwn
+  · intro p
+    rw [←h₇']
+    simp [-DState.tr_eq_some_iff]
+    constructor <;> rintro ⟨sa, H₁, H₂, H₂'⟩
+    · use sa.setHist # p :: s.hist
+      have H₅ : sys.tr sd' p = some (sa.setHist # p :: sd'.hist)
+      · rw [←H₆]
+        simp [-DState.tr_eq_some_iff]
+        use sa
+      apply and_of
+      · rw [←h₇]
+        simp [-DState.tr_eq_some_iff]
+        use sa.setHist # p :: sd'.hist, H₅
+        rfl
+      intro H₄
+      simp
+      have hsa := AState.of_tr H₁
+      have H₇ := sys.wf_of_tr H₅
+      have H₈ : sys.WF # s.setHist sd'.hist; simp [h₇', hsd'.wf]
+      simp [State.dwn_setHist]
+      use H₂
+      rw [←H₃]
+      have H₉ : sys.WF # sd.setHist s.hist; simp [H₃, hs.wf]
+      rwa [State.dwn_setHist]
+    · use sa.setHist # p :: sd.hist
+      apply and_of
+      · rw [←H₃']
+        simp [-DState.tr_eq_some_iff]
+        use sa.setHist # p :: s.hist
+        simp [-DState.tr_eq_some_iff]
+        rwa [State.setHist_eq_self_of # hist_eq_of_tr H₁]
+      intro H₄
+      have hsa := AState.of_tr H₁
+      have H₇ := sys.wf_of_tr H₄
+      have H₈ : sys.WF # s.setHist sd'.hist; simp [h₇', hsd'.wf]
+      simp [State.dwn_setHist]
+      simp at H₂'
+      have G₁ : sys.WF # sa.setHist # p :: sd'.hist
+      · apply sys.wf_of_tr (a := sd') (t := p)
+        rw [←H₆]
+        simp [-DState.tr_eq_some_iff]
+        exact ⟨_, H₄, rfl⟩
+      rw [State.dwn_setHist] at H₂'
+      simp at H₂; use H₂
+      rw [←H₃']
+      have G₂ : sys.WF # s.setHist sd.hist
+      · simp [H₃', hsd.wf]
+      rwa [State.dwn_setHist]
+  split_ifs with h₉
+  · have H₁ := h₉; simp [-DState.tr_eq_some_iff, ←h₈] at H₁
+    simp [-DState.tr_eq_some_iff, H₁]
+    simp [-DState.tr_eq_some_iff, h₈]
+  · have H₁ := h₉; simp_rw [←h₈] at H₁
+    simp [-DState.tr_eq_some_iff, H₁]
+
+@[simp]
+instance : dHistBlind.HistBlind := histBlind_dHistBlind
+
+theorem d_hws_and_dwn_lt_of_dHistBlind_tr {sd sa} [hsd : DState sd]
+(h₁ : sys.tr sd (dHistBlind.f sd) = some sa) (h₂ : sd.d_hws) :
+sa.d_hws ∧ sa.dwn < sd.dwn := by
+  simp [-DState.tr_eq_some_iff, dHistBlind, choose?_eq_ite] at h₁
+  
+  have h₃ : ∃ (sd' : State), sys.WF sd' ∧ sd'.setHist sd.hist = sd
+  · use sd; simp [hsd.wf]
+  have h₅ := Classical.epsilon_spec h₃
+  generalize h₄ : Classical.epsilon (λ (sd' : State) =>
+    sys.WF sd' ∧ sd'.setHist sd.hist = sd) = sd' at h₁ h₅
+  rcases h₅ with ⟨hsd', h₅⟩
+  
+  have h₆ : ∃ p sa, sys.tr sd' p = some sa ∧ sa.d_hws ∧ sa.dwn < sd'.dwn
+  · sorry
+  have h₇ := Classical.epsilon_spec h₆
+  generalize h₈ : Classical.epsilon (λ p => ∃ sa,
+    sys.tr sd' p = some sa ∧ sa.d_hws ∧ sa.dwn < sd'.dwn) = p at h₁ h₇
+  rcases h₇ with ⟨sa', h₇, h₉, H⟩
+  
+  have h₅' := setHist_eq_comm.mp h₅
+  
+  have H₁ : sys.tr sd p = sa'.setHist (p :: sd.hist)
+  · clear h₁
+    rw [←h₅'] at h₇
+    simp [-DState.tr_eq_some_iff] at h₇
+    obtain ⟨sa', h₇, rfl⟩ := h₇
+    simp [-DState.tr_eq_some_iff]
+    rwa [State.setHist_eq_self_of]
+    exact hist_eq_of_tr h₇
+  
+  have H₁' : sys.validTr sd p := ⟨_, H₁⟩
+  
+  have H₂ : sa.setHist sa'.hist = sa'
+  · clear h₁
+    rw [←h₅'] at h₇
+    sorry
+  
+  simp [-DState.tr_eq_some_iff, h₃, h₆, h₈, H₁'] at h₁
+  
+  constructor
+  · sorry
+  · sorry
+
 -- #check 0 #exit
 
 theorem State.d_hws_histBlind_of_d_hws {s} [hs : sys.WF s] (h : s.d_hws) :
-∃ (d : DStrat), d.WF ∧ d.histBlind ∧ ∀ (a : AStrat), a.WF → s.d_wins ⟨a, d⟩ := by
-  sorry
+∃ (d : DStrat), d.HistBlind ∧ ∀ (a : AStrat), a.WF → s.d_wins ⟨a, d⟩ := by
+  use dHistBlind, inferInstance
+  intro a Ha
+  apply d_wins_of_lt_lt (p := (·.d_hws)) (f := (·.dwn)) h <;> clear! s
+  · intro sa sd hsa hsd h₁ h₂
+    use hsa.d_hws_of_tr h₂ h₁, hsa.dwn_lt_of_tr h₁ h₂
+  · intro sd sa hsd hsa h₁ h₂
+    exact d_hws_and_dwn_lt_of_dHistBlind_tr h₂ h₁
 
 -- #check 0 #exit
 
 theorem State.d_hws_iff_d_hws_histBlind {s} [hs : sys.WF s] : s.d_hws ↔
-∃ (d : DStrat), d.WF ∧ d.histBlind ∧ ∀ (a : AStrat), a.WF → s.d_wins ⟨a, d⟩ :=
-  ⟨d_hws_histBlind_of_d_hws, λ ⟨d, Hd, h₁, h₂⟩ => by use d⟩
+∃ (d : DStrat), d.HistBlind ∧ ∀ (a : AStrat), a.WF → s.d_wins ⟨a, d⟩ :=
+  ⟨d_hws_histBlind_of_d_hws, λ ⟨d, Hd, h₁⟩ => by use d, Hd.wf⟩
