AP/AP/HistBlind/Defs.lean
@@ -2,10 +2,12 @@ import AP.AP.Bounded
 
 namespace AP
 
-def AStrat.histBlind (a : AStrat) : Prop :=
-  ∀ s hist, AState s → sys.WF (s.setHist hist) →
-  sys.hasTr s → a.f (s.setHist hist) = a.f s
+class AStrat.HistBlind (a : AStrat) : Prop where
+  wf : a.WF
+  h : ∀ s hist, AState s → sys.WF (s.setHist hist) →
+    sys.hasTr s → a.f (s.setHist hist) = a.f s
 
-def DStrat.histBlind (d : DStrat) : Prop :=
-  ∀ s hist, DState s → sys.WF (s.setHist hist) →
-  sys.hasTr s → d.f (s.setHist hist) = d.f s
+class DStrat.HistBlind (d : DStrat) : Prop where
+  wf : d.WF
+  h : ∀ s hist, DState s → sys.WF (s.setHist hist) →
+    sys.hasTr s → d.f (s.setHist hist) = d.f s
