AP/AP/HistBlind/Basic.lean
@@ -1,3 +1,22 @@
 import AP.AP.HistBlind.Defs
 
 namespace AP
+
+theorem AStrat.histBlind_def {a : AStrat} :
+a.HistBlind ↔ a.WF ∧ ∀ s hist, AState s → sys.WF (s.setHist hist) →
+sys.hasTr s → a.f (s.setHist hist) = a.f s :=
+  ⟨λ ⟨h₁, h₂⟩ => ⟨h₁, h₂⟩, λ ⟨h₁, h₂⟩ => ⟨h₁, h₂⟩⟩
+
+theorem DStrat.histBlind_def {d : DStrat} :
+d.HistBlind ↔ d.WF ∧ ∀ s hist, DState s → sys.WF (s.setHist hist) →
+sys.hasTr s → d.f (s.setHist hist) = d.f s :=
+  ⟨λ ⟨h₁, h₂⟩ => ⟨h₁, h₂⟩, λ ⟨h₁, h₂⟩ => ⟨h₁, h₂⟩⟩
+
+instance {a : AStrat} [ha : a.HistBlind] : a.WF := ha.wf
+instance {d : DStrat} [hd : d.HistBlind] : d.WF := hd.wf
+
+instance : (default : AStrat).HistBlind := by
+  simp [AStrat.histBlind_def]; infer_instance
+
+instance : (default : DStrat).HistBlind := by
+  simp [DStrat.histBlind_def]; infer_instance
